program_logic/auth.v
@@ -83,24 +83,28 @@ Section auth.
   (* Notice how the user has to prove that `b⋅a'` is valid at all
      step-indices. However, since A is timeless, that should not be
      a restriction.  *)
-  Lemma auth_fsa {X : Type} {FSA} (FSAs : FrameShiftAssertion (A:=X) FSA)
-        L `{!LocalUpdate Lv L} N E P (Q : X → iPropG Λ Σ) γ a :
+  Lemma auth_fsa {B} (fsa : FSA Λ (globalF Σ) B) `{!FrameShiftAssertion fsaV fsa}
+       L `{!LocalUpdate Lv L} N E P (Q : B → iPropG Λ Σ) γ a :
+    fsaV →
     nclose N ⊆ E →
     P ⊑ auth_ctx AuthI γ N φ →
-    P ⊑ (auth_own AuthI γ a ★ (∀ a', ■✓(a ⋅ a') ★ ▷φ (a ⋅ a') -★
-        FSA (E ∖ nclose N) (λ x, ■(Lv a ∧ ✓(L a⋅a')) ★ ▷φ (L a ⋅ a') ★ (auth_own AuthI γ (L a) -★ Q x)))) →
-    P ⊑ FSA E Q.
+    P ⊑ (auth_own AuthI γ a ★ (∀ a',
+          ■ ✓ (a ⋅ a') ★ ▷ φ (a ⋅ a') -★
+          fsa (E ∖ nclose N) (λ x,
+            ■ (Lv a ∧ ✓(L a⋅a')) ★ ▷ φ (L a ⋅ a') ★
+            (auth_own AuthI γ (L a) -★ Q x)))) →
+    P ⊑ fsa E Q.
   Proof.
-    rewrite /auth_ctx=>HN Hinv Hinner.
-    eapply inv_fsa; [eassumption..|]. rewrite Hinner=>{Hinner Hinv P}.
+    rewrite /auth_ctx=>? HN Hinv Hinner.
+    eapply (inv_fsa fsa); eauto. rewrite Hinner=>{Hinner Hinv P}.
     apply wand_intro_l.
     rewrite assoc auth_opened !pvs_frame_r !sep_exist_r.
-    apply fsa_strip_pvs; first done. apply exist_elim=>a'.
+    apply (fsa_strip_pvs fsa). apply exist_elim=>a'.
     rewrite (forall_elim a'). rewrite [(▷_ ★ _)%I]comm.
     (* Getting this wand eliminated is really annoying. *)
     rewrite [(■_ ★ _)%I]comm -!assoc [(▷φ _ ★ _ ★ _)%I]assoc [(▷φ _ ★ _)%I]comm.
     rewrite wand_elim_r fsa_frame_l.
-    apply fsa_mono_pvs; first done. intros x. rewrite comm -!assoc.
+    apply (fsa_mono_pvs fsa)=> x. rewrite comm -!assoc.
     apply const_elim_sep_l=>-[HL Hv].
     rewrite assoc [(_ ★ (_ -★ _))%I]comm -assoc.
     rewrite auth_closing //; []. erewrite pvs_frame_l. apply pvs_mono.
